feat: Add branch key id supplier for hierarchical keyring (#150)

AwsCryptographicMaterialProviders/runtimes/java/src/main/smithy-generated/software/amazon/cryptography/materialProviders/BranchKeyIdSupplier.java
@@ -1,0 +1,81 @@
+// Copyright Amazon.com Inc. or its affiliates. All Rights Reserved.
+// SPDX-License-Identifier: Apache-2.0
+// Do not modify this file. This file is machine generated, and any changes to it will be overwritten.
+package software.amazon.cryptography.materialProviders;
+
+import Dafny.Aws.Cryptography.MaterialProviders.Types.Error;
+import Wrappers_Compile.Result;
+import java.lang.Exception;
+import java.lang.IllegalArgumentException;
+import java.util.Objects;
+import software.amazon.cryptography.materialProviders.model.GetBranchKeyIdInput;
+import software.amazon.cryptography.materialProviders.model.GetBranchKeyIdOutput;
+import software.amazon.cryptography.materialProviders.model.NativeError;
+import software.amazon.cryptography.materialProviders.model.OpaqueError;
+
+public final class BranchKeyIdSupplier implements IBranchKeyIdSupplier {
+  private final Dafny.Aws.Cryptography.MaterialProviders.Types.IBranchKeyIdSupplier _impl;
+
+  private BranchKeyIdSupplier(
+      Dafny.Aws.Cryptography.MaterialProviders.Types.IBranchKeyIdSupplier iBranchKeyIdSupplier) {
+    Objects.requireNonNull(iBranchKeyIdSupplier, "Missing value for required argument `iBranchKeyIdSupplier`");
+    this._impl = iBranchKeyIdSupplier;
+  }
+
+  public static BranchKeyIdSupplier wrap(
+      Dafny.Aws.Cryptography.MaterialProviders.Types.IBranchKeyIdSupplier iBranchKeyIdSupplier) {
+    return new BranchKeyIdSupplier(iBranchKeyIdSupplier);
+  }
+
+  public static <I extends IBranchKeyIdSupplier> BranchKeyIdSupplier wrap(I iBranchKeyIdSupplier) {
+    Objects.requireNonNull(iBranchKeyIdSupplier, "Missing value for required argument `iBranchKeyIdSupplier`");
+    if (iBranchKeyIdSupplier instanceof software.amazon.cryptography.materialProviders.BranchKeyIdSupplier) {
+      return ((BranchKeyIdSupplier) iBranchKeyIdSupplier);
+    }
+    return BranchKeyIdSupplier.wrap(new NativeWrapper(iBranchKeyIdSupplier));
+  }
+
+  public Dafny.Aws.Cryptography.MaterialProviders.Types.IBranchKeyIdSupplier impl() {
+    return this._impl;
+  }
+
+  public GetBranchKeyIdOutput GetBranchKeyId(GetBranchKeyIdInput nativeValue) {
+    Dafny.Aws.Cryptography.MaterialProviders.Types.GetBranchKeyIdInput dafnyValue = ToDafny.GetBranchKeyIdInput(nativeValue);
+    Result<Dafny.Aws.Cryptography.MaterialProviders.Types.GetBranchKeyIdOutput, Error> result = this._impl.GetBranchKeyId(dafnyValue);
+    if (result.is_Failure()) {
+      throw ToNative.Error(result.dtor_error());
+    }
+    return ToNative.GetBranchKeyIdOutput(result.dtor_value());
+  }
+
+  private static final class NativeWrapper implements Dafny.Aws.Cryptography.MaterialProviders.Types.IBranchKeyIdSupplier {
+    private final IBranchKeyIdSupplier _impl;
+
+    NativeWrapper(IBranchKeyIdSupplier nativeImpl) {
+      if (nativeImpl instanceof BranchKeyIdSupplier) {
+        throw new IllegalArgumentException("Recursive wrapping is strictly forbidden.");
+      }
+      this._impl = nativeImpl;
+    }
+
+    public Result<Dafny.Aws.Cryptography.MaterialProviders.Types.GetBranchKeyIdOutput, Error> GetBranchKeyId(
+        Dafny.Aws.Cryptography.MaterialProviders.Types.GetBranchKeyIdInput dafnyInput) {
+      GetBranchKeyIdInput nativeInput = ToNative.GetBranchKeyIdInput(dafnyInput);
+      try {
+        GetBranchKeyIdOutput nativeOutput = this._impl.GetBranchKeyId(nativeInput);
+        Dafny.Aws.Cryptography.MaterialProviders.Types.GetBranchKeyIdOutput dafnyOutput = ToDafny.GetBranchKeyIdOutput(nativeOutput);
+        return Result.create_Success(dafnyOutput);
+      } catch (NativeError ex) {
+        return Result.create_Failure(ToDafny.Error(ex));
+      } catch (Exception ex) {
+        OpaqueError error = OpaqueError.builder().obj(ex).cause(ex).build();
+        return Result.create_Failure(ToDafny.Error(error));
+      }
+    }
+
+    public Result<Dafny.Aws.Cryptography.MaterialProviders.Types.GetBranchKeyIdOutput, Error> GetBranchKeyId_k(
+        Dafny.Aws.Cryptography.MaterialProviders.Types.GetBranchKeyIdInput dafnyInput) {
+      throw NativeError.builder().message("Not supported at this time.").build();
+    }
+  }
+}
