AwsCryptographicMaterialProviders/runtimes/java/src/main/smithy-generated/software/amazon/cryptography/materialProviders/model/GetBranchKeyIdInput.java
@@ -1,0 +1,62 @@
+// Copyright Amazon.com Inc. or its affiliates. All Rights Reserved.
+// SPDX-License-Identifier: Apache-2.0
+// Do not modify this file. This file is machine generated, and any changes to it will be overwritten.
+package software.amazon.cryptography.materialProviders.model;
+
+import java.util.Map;
+import java.util.Objects;
+
+public class GetBranchKeyIdInput {
+  private final Map<String, String> encryptionContext;
+
+  protected GetBranchKeyIdInput(BuilderImpl builder) {
+    this.encryptionContext = builder.encryptionContext();
+  }
+
+  public Map<String, String> encryptionContext() {
+    return this.encryptionContext;
+  }
+
+  public Builder toBuilder() {
+    return new BuilderImpl(this);
+  }
+
+  public static Builder builder() {
+    return new BuilderImpl();
+  }
+
+  public interface Builder {
+    Builder encryptionContext(Map<String, String> encryptionContext);
+
+    Map<String, String> encryptionContext();
+
+    GetBranchKeyIdInput build();
+  }
+
+  static class BuilderImpl implements Builder {
+    protected Map<String, String> encryptionContext;
+
+    protected BuilderImpl() {
+    }
+
+    protected BuilderImpl(GetBranchKeyIdInput model) {
+      this.encryptionContext = model.encryptionContext();
+    }
+
+    public Builder encryptionContext(Map<String, String> encryptionContext) {
+      this.encryptionContext = encryptionContext;
+      return this;
+    }
+
+    public Map<String, String> encryptionContext() {
+      return this.encryptionContext;
+    }
+
+    public GetBranchKeyIdInput build() {
+      if (Objects.isNull(this.encryptionContext()))  {
+        throw new IllegalArgumentException("Missing value for required field `encryptionContext`");
+      }
+      return new GetBranchKeyIdInput(this);
+    }
+  }
+}
