AwsCryptographicMaterialProviders/runtimes/net/Generated/TypeConversion.cs
@@ -133,7 +133,8 @@ namespace AWS.Cryptography.MaterialProviders
     }
     internal static AWS.Cryptography.MaterialProviders.CreateAwsKmsHierarchicalKeyringInput FromDafny_N3_aws__N12_cryptography__N17_materialProviders__S36_CreateAwsKmsHierarchicalKeyringInput(Dafny.Aws.Cryptography.MaterialProviders.Types._ICreateAwsKmsHierarchicalKeyringInput value)
     {
-      Dafny.Aws.Cryptography.MaterialProviders.Types.CreateAwsKmsHierarchicalKeyringInput concrete = (Dafny.Aws.Cryptography.MaterialProviders.Types.CreateAwsKmsHierarchicalKeyringInput)value; AWS.Cryptography.MaterialProviders.CreateAwsKmsHierarchicalKeyringInput converted = new AWS.Cryptography.MaterialProviders.CreateAwsKmsHierarchicalKeyringInput(); converted.BranchKeyId = (string)FromDafny_N3_aws__N12_cryptography__N17_materialProviders__S36_CreateAwsKmsHierarchicalKeyringInput__M11_branchKeyId(concrete._branchKeyId);
+      Dafny.Aws.Cryptography.MaterialProviders.Types.CreateAwsKmsHierarchicalKeyringInput concrete = (Dafny.Aws.Cryptography.MaterialProviders.Types.CreateAwsKmsHierarchicalKeyringInput)value; AWS.Cryptography.MaterialProviders.CreateAwsKmsHierarchicalKeyringInput converted = new AWS.Cryptography.MaterialProviders.CreateAwsKmsHierarchicalKeyringInput(); if (concrete._branchKeyId.is_Some) converted.BranchKeyId = (string)FromDafny_N3_aws__N12_cryptography__N17_materialProviders__S36_CreateAwsKmsHierarchicalKeyringInput__M11_branchKeyId(concrete._branchKeyId);
+      if (concrete._branchKeyIdSupplier.is_Some) converted.BranchKeyIdSupplier = (AWS.Cryptography.MaterialProviders.IBranchKeyIdSupplier)FromDafny_N3_aws__N12_cryptography__N17_materialProviders__S36_CreateAwsKmsHierarchicalKeyringInput__M19_branchKeyIdSupplier(concrete._branchKeyIdSupplier);
       converted.KmsKeyId = (string)FromDafny_N3_aws__N12_cryptography__N17_materialProviders__S36_CreateAwsKmsHierarchicalKeyringInput__M8_kmsKeyId(concrete._kmsKeyId);
       converted.KmsClient = (Amazon.KeyManagementService.IAmazonKeyManagementService)FromDafny_N3_aws__N12_cryptography__N17_materialProviders__S36_CreateAwsKmsHierarchicalKeyringInput__M9_kmsClient(concrete._kmsClient);
       converted.DdbClient = (Amazon.DynamoDBv2.IAmazonDynamoDB)FromDafny_N3_aws__N12_cryptography__N17_materialProviders__S36_CreateAwsKmsHierarchicalKeyringInput__M9_ddbClient(concrete._ddbClient);
@@ -144,9 +145,11 @@ namespace AWS.Cryptography.MaterialProviders
     }
     internal static Dafny.Aws.Cryptography.MaterialProviders.Types._ICreateAwsKmsHierarchicalKeyringInput ToDafny_N3_aws__N12_cryptography__N17_materialProviders__S36_CreateAwsKmsHierarchicalKeyringInput(AWS.Cryptography.MaterialProviders.CreateAwsKmsHierarchicalKeyringInput value)
     {
+      string var_branchKeyId = value.IsSetBranchKeyId() ? value.BranchKeyId : (string)null;
+      AWS.Cryptography.MaterialProviders.IBranchKeyIdSupplier var_branchKeyIdSupplier = value.IsSetBranchKeyIdSupplier() ? value.BranchKeyIdSupplier : (AWS.Cryptography.MaterialProviders.IBranchKeyIdSupplier)null;
       int? var_maxCacheSize = value.IsSetMaxCacheSize() ? value.MaxCacheSize : (int?)null;
       System.Collections.Generic.List<string> var_grantTokens = value.IsSetGrantTokens() ? value.GrantTokens : (System.Collections.Generic.List<string>)null;
-      return new Dafny.Aws.Cryptography.MaterialProviders.Types.CreateAwsKmsHierarchicalKeyringInput(ToDafny_N3_aws__N12_cryptography__N17_materialProviders__S36_CreateAwsKmsHierarchicalKeyringInput__M11_branchKeyId(value.BranchKeyId), ToDafny_N3_aws__N12_cryptography__N17_materialProviders__S36_CreateAwsKmsHierarchicalKeyringInput__M8_kmsKeyId(value.KmsKeyId), ToDafny_N3_aws__N12_cryptography__N17_materialProviders__S36_CreateAwsKmsHierarchicalKeyringInput__M9_kmsClient(value.KmsClient), ToDafny_N3_aws__N12_cryptography__N17_materialProviders__S36_CreateAwsKmsHierarchicalKeyringInput__M9_ddbClient(value.DdbClient), ToDafny_N3_aws__N12_cryptography__N17_materialProviders__S36_CreateAwsKmsHierarchicalKeyringInput__M17_branchKeyStoreArn(value.BranchKeyStoreArn), ToDafny_N3_aws__N12_cryptography__N17_materialProviders__S36_CreateAwsKmsHierarchicalKeyringInput__M10_ttlSeconds(value.TtlSeconds), ToDafny_N3_aws__N12_cryptography__N17_materialProviders__S36_CreateAwsKmsHierarchicalKeyringInput__M12_maxCacheSize(var_maxCacheSize), ToDafny_N3_aws__N12_cryptography__N17_materialProviders__S36_CreateAwsKmsHierarchicalKeyringInput__M11_grantTokens(var_grantTokens));
+      return new Dafny.Aws.Cryptography.MaterialProviders.Types.CreateAwsKmsHierarchicalKeyringInput(ToDafny_N3_aws__N12_cryptography__N17_materialProviders__S36_CreateAwsKmsHierarchicalKeyringInput__M11_branchKeyId(var_branchKeyId), ToDafny_N3_aws__N12_cryptography__N17_materialProviders__S36_CreateAwsKmsHierarchicalKeyringInput__M19_branchKeyIdSupplier(var_branchKeyIdSupplier), ToDafny_N3_aws__N12_cryptography__N17_materialProviders__S36_CreateAwsKmsHierarchicalKeyringInput__M8_kmsKeyId(value.KmsKeyId), ToDafny_N3_aws__N12_cryptography__N17_materialProviders__S36_CreateAwsKmsHierarchicalKeyringInput__M9_kmsClient(value.KmsClient), ToDafny_N3_aws__N12_cryptography__N17_materialProviders__S36_CreateAwsKmsHierarchicalKeyringInput__M9_ddbClient(value.DdbClient), ToDafny_N3_aws__N12_cryptography__N17_materialProviders__S36_CreateAwsKmsHierarchicalKeyringInput__M17_branchKeyStoreArn(value.BranchKeyStoreArn), ToDafny_N3_aws__N12_cryptography__N17_materialProviders__S36_CreateAwsKmsHierarchicalKeyringInput__M10_ttlSeconds(value.TtlSeconds), ToDafny_N3_aws__N12_cryptography__N17_materialProviders__S36_CreateAwsKmsHierarchicalKeyringInput__M12_maxCacheSize(var_maxCacheSize), ToDafny_N3_aws__N12_cryptography__N17_materialProviders__S36_CreateAwsKmsHierarchicalKeyringInput__M11_grantTokens(var_grantTokens));
     }
     internal static AWS.Cryptography.MaterialProviders.CreateAwsKmsKeyringInput FromDafny_N3_aws__N12_cryptography__N17_materialProviders__S24_CreateAwsKmsKeyringInput(Dafny.Aws.Cryptography.MaterialProviders.Types._ICreateAwsKmsKeyringInput value)
     {
@@ -602,6 +605,24 @@ namespace AWS.Cryptography.MaterialProviders
     internal static Dafny.ISequence<byte> ToDafny_N3_aws__N12_cryptography__N17_materialProviders__S26_GetAlgorithmSuiteInfoInput(System.IO.MemoryStream value)
     {
       return ToDafny_N3_aws__N12_cryptography__N17_materialProviders__S26_GetAlgorithmSuiteInfoInput__M8_binaryId(value);
+    }
+    internal static AWS.Cryptography.MaterialProviders.GetBranchKeyIdInput FromDafny_N3_aws__N12_cryptography__N17_materialProviders__S19_GetBranchKeyIdInput(Dafny.Aws.Cryptography.MaterialProviders.Types._IGetBranchKeyIdInput value)
+    {
+      Dafny.Aws.Cryptography.MaterialProviders.Types.GetBranchKeyIdInput concrete = (Dafny.Aws.Cryptography.MaterialProviders.Types.GetBranchKeyIdInput)value; AWS.Cryptography.MaterialProviders.GetBranchKeyIdInput converted = new AWS.Cryptography.MaterialProviders.GetBranchKeyIdInput(); converted.EncryptionContext = (System.Collections.Generic.Dictionary<string, string>)FromDafny_N3_aws__N12_cryptography__N17_materialProviders__S19_GetBranchKeyIdInput__M17_encryptionContext(concrete._encryptionContext); return converted;
+    }
+    internal static Dafny.Aws.Cryptography.MaterialProviders.Types._IGetBranchKeyIdInput ToDafny_N3_aws__N12_cryptography__N17_materialProviders__S19_GetBranchKeyIdInput(AWS.Cryptography.MaterialProviders.GetBranchKeyIdInput value)
+    {
+
+      return new Dafny.Aws.Cryptography.MaterialProviders.Types.GetBranchKeyIdInput(ToDafny_N3_aws__N12_cryptography__N17_materialProviders__S19_GetBranchKeyIdInput__M17_encryptionContext(value.EncryptionContext));
+    }
+    internal static AWS.Cryptography.MaterialProviders.GetBranchKeyIdOutput FromDafny_N3_aws__N12_cryptography__N17_materialProviders__S20_GetBranchKeyIdOutput(Dafny.Aws.Cryptography.MaterialProviders.Types._IGetBranchKeyIdOutput value)
+    {
+      Dafny.Aws.Cryptography.MaterialProviders.Types.GetBranchKeyIdOutput concrete = (Dafny.Aws.Cryptography.MaterialProviders.Types.GetBranchKeyIdOutput)value; AWS.Cryptography.MaterialProviders.GetBranchKeyIdOutput converted = new AWS.Cryptography.MaterialProviders.GetBranchKeyIdOutput(); converted.BranchKeyId = (string)FromDafny_N3_aws__N12_cryptography__N17_materialProviders__S20_GetBranchKeyIdOutput__M11_branchKeyId(concrete._branchKeyId); return converted;
+    }
+    internal static Dafny.Aws.Cryptography.MaterialProviders.Types._IGetBranchKeyIdOutput ToDafny_N3_aws__N12_cryptography__N17_materialProviders__S20_GetBranchKeyIdOutput(AWS.Cryptography.MaterialProviders.GetBranchKeyIdOutput value)
+    {
+
+      return new Dafny.Aws.Cryptography.MaterialProviders.Types.GetBranchKeyIdOutput(ToDafny_N3_aws__N12_cryptography__N17_materialProviders__S20_GetBranchKeyIdOutput__M11_branchKeyId(value.BranchKeyId));
     }
     internal static AWS.Cryptography.MaterialProviders.GetCacheEntryInput FromDafny_N3_aws__N12_cryptography__N17_materialProviders__S18_GetCacheEntryInput(Dafny.Aws.Cryptography.MaterialProviders.Types._IGetCacheEntryInput value)
     {
@@ -1170,13 +1191,21 @@ namespace AWS.Cryptography.MaterialProviders
     {
       return value == null ? Wrappers_Compile.Option<Dafny.ISequence<Dafny.ISequence<char>>>.create_None() : Wrappers_Compile.Option<Dafny.ISequence<Dafny.ISequence<char>>>.create_Some(ToDafny_N3_aws__N12_cryptography__N17_materialProviders__S14_GrantTokenList((System.Collections.Generic.List<string>)value));
     }
-    internal static string FromDafny_N3_aws__N12_cryptography__N17_materialProviders__S36_CreateAwsKmsHierarchicalKeyringInput__M11_branchKeyId(Dafny.ISequence<char> value)
+    internal static string FromDafny_N3_aws__N12_cryptography__N17_materialProviders__S36_CreateAwsKmsHierarchicalKeyringInput__M11_branchKeyId(Wrappers_Compile._IOption<Dafny.ISequence<char>> value)
     {
-      return FromDafny_N6_smithy__N3_api__S6_String(value);
+      return value.is_None ? (string)null : FromDafny_N6_smithy__N3_api__S6_String(value.Extract());
     }
-    internal static Dafny.ISequence<char> ToDafny_N3_aws__N12_cryptography__N17_materialProviders__S36_CreateAwsKmsHierarchicalKeyringInput__M11_branchKeyId(string value)
+    internal static Wrappers_Compile._IOption<Dafny.ISequence<char>> ToDafny_N3_aws__N12_cryptography__N17_materialProviders__S36_CreateAwsKmsHierarchicalKeyringInput__M11_branchKeyId(string value)
     {
-      return ToDafny_N6_smithy__N3_api__S6_String(value);
+      return value == null ? Wrappers_Compile.Option<Dafny.ISequence<char>>.create_None() : Wrappers_Compile.Option<Dafny.ISequence<char>>.create_Some(ToDafny_N6_smithy__N3_api__S6_String((string)value));
+    }
+    internal static AWS.Cryptography.MaterialProviders.IBranchKeyIdSupplier FromDafny_N3_aws__N12_cryptography__N17_materialProviders__S36_CreateAwsKmsHierarchicalKeyringInput__M19_branchKeyIdSupplier(Wrappers_Compile._IOption<Dafny.Aws.Cryptography.MaterialProviders.Types.IBranchKeyIdSupplier> value)
+    {
+      return value.is_None ? (AWS.Cryptography.MaterialProviders.IBranchKeyIdSupplier)null : FromDafny_N3_aws__N12_cryptography__N17_materialProviders__S28_BranchKeyIdSupplierReference(value.Extract());
+    }
+    internal static Wrappers_Compile._IOption<Dafny.Aws.Cryptography.MaterialProviders.Types.IBranchKeyIdSupplier> ToDafny_N3_aws__N12_cryptography__N17_materialProviders__S36_CreateAwsKmsHierarchicalKeyringInput__M19_branchKeyIdSupplier(AWS.Cryptography.MaterialProviders.IBranchKeyIdSupplier value)
+    {
+      return value == null ? Wrappers_Compile.Option<Dafny.Aws.Cryptography.MaterialProviders.Types.IBranchKeyIdSupplier>.create_None() : Wrappers_Compile.Option<Dafny.Aws.Cryptography.MaterialProviders.Types.IBranchKeyIdSupplier>.create_Some(ToDafny_N3_aws__N12_cryptography__N17_materialProviders__S28_BranchKeyIdSupplierReference((AWS.Cryptography.MaterialProviders.IBranchKeyIdSupplier)value));
     }
     internal static string FromDafny_N3_aws__N12_cryptography__N17_materialProviders__S36_CreateAwsKmsHierarchicalKeyringInput__M8_kmsKeyId(Dafny.ISequence<char> value)
     {
@@ -1858,6 +1887,22 @@ namespace AWS.Cryptography.MaterialProviders
     {
       return ToDafny_N6_smithy__N3_api__S4_Blob(value);
     }
+    internal static System.Collections.Generic.Dictionary<string, string> FromDafny_N3_aws__N12_cryptography__N17_materialProviders__S19_GetBranchKeyIdInput__M17_encryptionContext(Dafny.IMap<Dafny.ISequence<byte>, Dafny.ISequence<byte>> value)
+    {
+      return FromDafny_N3_aws__N12_cryptography__N17_materialProviders__S17_EncryptionContext(value);
+    }
+    internal static Dafny.IMap<Dafny.ISequence<byte>, Dafny.ISequence<byte>> ToDafny_N3_aws__N12_cryptography__N17_materialProviders__S19_GetBranchKeyIdInput__M17_encryptionContext(System.Collections.Generic.Dictionary<string, string> value)
+    {
+      return ToDafny_N3_aws__N12_cryptography__N17_materialProviders__S17_EncryptionContext(value);
+    }
+    internal static string FromDafny_N3_aws__N12_cryptography__N17_materialProviders__S20_GetBranchKeyIdOutput__M11_branchKeyId(Dafny.ISequence<char> value)
+    {
+      return FromDafny_N6_smithy__N3_api__S6_String(value);
+    }
+    internal static Dafny.ISequence<char> ToDafny_N3_aws__N12_cryptography__N17_materialProviders__S20_GetBranchKeyIdOutput__M11_branchKeyId(string value)
+    {
+      return ToDafny_N6_smithy__N3_api__S6_String(value);
+    }
     internal static System.IO.MemoryStream FromDafny_N3_aws__N12_cryptography__N17_materialProviders__S18_GetCacheEntryInput__M10_identifier(Dafny.ISequence<byte> value)
     {
       return FromDafny_N6_smithy__N3_api__S4_Blob(value);
@@ -2399,6 +2444,25 @@ namespace AWS.Cryptography.MaterialProviders
         default:
           throw new System.ArgumentException(
               "Custom implementations of ClientSupplier must extend ClientSupplierBase.");
+      }
+    }
+    public static AWS.Cryptography.MaterialProviders.IBranchKeyIdSupplier FromDafny_N3_aws__N12_cryptography__N17_materialProviders__S28_BranchKeyIdSupplierReference(Dafny.Aws.Cryptography.MaterialProviders.Types.IBranchKeyIdSupplier value)
+    {
+      if (value is NativeWrapper_BranchKeyIdSupplier nativeWrapper) return nativeWrapper._impl;
+      return new BranchKeyIdSupplier(value);
+
+    }
+    public static Dafny.Aws.Cryptography.MaterialProviders.Types.IBranchKeyIdSupplier ToDafny_N3_aws__N12_cryptography__N17_materialProviders__S28_BranchKeyIdSupplierReference(AWS.Cryptography.MaterialProviders.IBranchKeyIdSupplier value)
+    {
+      switch (value)
+      {
+        case BranchKeyIdSupplier valueWithImpl:
+          return valueWithImpl._impl;
+        case BranchKeyIdSupplierBase nativeImpl:
+          return new NativeWrapper_BranchKeyIdSupplier(nativeImpl);
+        default:
+          throw new System.ArgumentException(
+              "Custom implementations of BranchKeyIdSupplier must extend BranchKeyIdSupplierBase.");
       }
     }
     internal static string FromDafny_N3_aws__N12_cryptography__N17_materialProviders__S8_KmsKeyId(Dafny.ISequence<char> value)
